

Seminar 2: OLS Properties

Unbiasedness, Variance, and Standard Errors

Giulio Rossetti*

giuliorossetti94.github.io

January 30, 2026

* email: giulio.rossetti.1@wbs.ac.uk

Roadmap

Part 1: OLS Unbiasedness

Exercise 1: Unbiasedness

Exercise 2: Variance of OLS Estimator

Part 2: Collinearity

Exercise 2.2-2.3: Collinearity and Irrelevant Variables

Roadmap

Part 1: OLS Unbiasedness

Exercise 1: Unbiasedness

Exercise 2: Variance of OLS Estimator

Part 2: Collinearity

Exercise 2.2-2.3: Collinearity and Irrelevant Variables

Unbiasedness

Definition

An estimator of a given parameter is said to be **unbiased** if its expected value is equal to the true value of the parameter:

$$\mathbb{E}[\hat{\theta}(\xi)] = \theta_0$$

OLS unbiasedness (Exercise 1)

- OLS Assumptions:
 1. Linear in parameters
 2. Random sampling
 3. No perfect collinearity
 4. Zero conditional mean: $E[u_i|x_i] = E[u_i] = 0$.
- Under assumptions 1-4 the OLS estimator is unbiased

$$E[\hat{\beta}] = \beta$$

OLS unbiasedness: proof

Variance of OLS estimator: derivation (Exercise 2)

5. Homoskedasticity: $Var(\mathbf{u}|\mathbf{X}) = \sigma^2 \mathbf{I}_n$ $\sigma^2 > 0$

Variance of OLS estimates

- The variance of the OLS estimates is given by:

$$\text{Var}(\hat{\beta}|\mathbf{X}) = \sigma^2(\mathbf{X}'\mathbf{X})^{-1}$$

- The standard errors are given by:

$$se(\hat{\beta}_j) = \sqrt{\text{Var}(\hat{\beta}_j | \mathbf{X})} = \sqrt{\sigma^2 (\mathbf{X}'\mathbf{X})_{jj}^{-1}} = \sigma \sqrt{(\mathbf{X}'\mathbf{X})_{jj}^{-1}}.$$

- σ^2 is not observed. Obtain an unbiased estimate through the OLS residuals $\hat{\mathbf{u}} = \mathbf{y} - \mathbf{X}\hat{\beta}$

Variance of OLS estimates

- then

$$\hat{\sigma}^2 = \frac{\hat{\mathbf{u}}' \hat{\mathbf{u}}}{n - k - 1},$$

- therefore,

$$se(\hat{\beta}_j) = \hat{\sigma} \sqrt{(\mathbf{X}'\mathbf{X})_{jj}^{-1}}.$$

- Increasing the sample size n reduces $\hat{\sigma}^2$ and hence the standard errors.

SE of OLS estimates: SLR and matrices (Exercise 5)

- In the SLR case, \mathbf{X} is a $n \times 2$ matrix:

$$\mathbf{X} = \begin{bmatrix} 1 & x_1 \\ 1 & x_2 \\ \vdots & \vdots \\ 1 & x_n \end{bmatrix}$$

- then $\mathbf{X}'\mathbf{X}$ is a 2×2 matrix:

$$\mathbf{X}'\mathbf{X} = \begin{bmatrix} n & \sum x_i \\ \sum x_i & \sum x_i^2 \end{bmatrix}$$

- and its inverse is (see matrix algebra slides):

$$(\mathbf{X}'\mathbf{X})^{-1} = \frac{1}{n \sum x_i^2 - (\sum x_i)^2} \begin{bmatrix} \sum x_i^2 & -\sum x_i \\ -\sum x_i & n \end{bmatrix}$$

SE of OLS estimates: SLR and matrices (Exercise 5)

- to compute the standard errors we use the formula:

$$se(\hat{\beta}_j) = \hat{\sigma} \sqrt{(\mathbf{X}'\mathbf{X})_{jj}^{-1}}.$$

- therefore, the standard errors for $\hat{\beta}_0$ and $\hat{\beta}_1$ are:

$$se(\hat{\beta}_0) = \hat{\sigma} \sqrt{\frac{\sum x_i^2}{n \sum x_i^2 - (\sum x_i)^2}}$$

$$se(\hat{\beta}_1) = \hat{\sigma} \sqrt{\frac{n}{n \sum x_i^2 - (\sum x_i)^2}}$$

Exercise 1

Standard Errors of OLS Estimates

Model:

$$Wage = \beta_0 + \beta_1 Educ + u$$

- $\hat{\beta}_1 = 1.04, \quad \hat{\beta}_0 = -6.90.$
- $\hat{\sigma}^2 = \frac{1}{n-2} \sum_{i=1}^n \hat{u}_i^2 = 10.31.$

$$\text{Var}(\hat{\beta}_0) = 19.54 \implies \text{se}(\hat{\beta}_0) = 4.42.$$

$$\text{Var}(\hat{\beta}_1) = 0.108 \implies \text{se}(\hat{\beta}_1) = 0.33.$$

Roadmap

Part 1: OLS Unbiasedness

Exercise 1: Unbiasedness

Exercise 2: Variance of OLS Estimator

Part 2: Collinearity

Exercise 2.2-2.3: Collinearity and Irrelevant Variables

Exercise 2.2-2.3

Collinearity

Model:

$$y_i = \beta_0 + \beta_1 x_{1,i} + \beta_2 x_{2,i} + \beta_3 x_{3,i} + u_i \quad i = 1, \dots, n$$

- **Collinearity:** If $x_3 = x_1 + x_2 + 6$, perfect collinearity exists, making OLS infeasible.
- assumption 3 is violated.
- rank of $\mathbf{X}'\mathbf{X}$ is 2, not 3. Cannot invert the matrix.

Exercise 2.2-2.3

Irrelevant Variables

True model:

$$y_i = \beta_0 + \beta_1 x_{1,i} + \beta_2 x_{2,i} + u_i \quad i = 1, \dots, n$$

Estimated model:

$$y_i = \beta_0 + \beta_1 x_{1,i} + \beta_2 x_{2,i} + \beta_3 x_{3,i} + u_i \quad i = 1, \dots, n$$

- **Irrelevant Variables:** Including irrelevant variables (e.g., x_3) does not affect the unbiasedness but reduces efficiency.

Roadmap

Appendix

Appendix: Proof of OLS Unbiasedness

1.1. EX1

- ① Linear in parameters $y = \beta_0 + \beta_1 x + u$
- ② Random sampling
- ③ No multicollinearity
- ④ Errors have zero conditional means $E[u_i | x_i] = 0 \Rightarrow E[u_i] = 0$

under 1-4 OLS estimates are unbiased: $E[\hat{\beta}_0] = \beta_0$, $E[\hat{\beta}_1] = \beta_1$

$$\begin{aligned} \hat{\beta}_1 &= \frac{\sum_{i=1}^n (x_i - \bar{x})(y_i - \bar{y})}{\sum_{i=1}^n (x_i - \bar{x})^2} \\ &= \frac{\sum_{i=1}^n (x_i - \bar{x})y_i}{\sum_{i=1}^n (x_i - \bar{x})^2} \quad \text{using ① } y_i = \beta_0 + \beta_1 x_i + u_i \\ &= \frac{\sum_{i=1}^n (x_i - \bar{x})(\beta_0 + \beta_1 x_i + u_i)}{\sum_{i=1}^n (x_i - \bar{x})^2} \\ &= \frac{\beta_0 \sum_{i=1}^n (x_i - \bar{x}) + \beta_1 \sum_{i=1}^n (x_i - \bar{x})x_i + \sum_{i=1}^n (x_i - \bar{x})u_i}{\sum_{i=1}^n (x_i - \bar{x})^2} \end{aligned}$$

$\sum_{i=1}^n (x_i - \bar{x}) = \sum_{i=1}^n x_i - \sum_{i=1}^n \bar{x} = \bar{x}_n - \bar{x}_n = 0$

Appendix: Variance of OLS Estimator

$$\hat{\beta}_0 = \bar{y} - \hat{\beta}_1 \bar{x} \quad \text{using } ① \quad y_i = \beta_0 + \beta_1 x_i + u_i \quad \bar{y} = E[y_i] = \beta_0 + E[\beta_1 x_i] + E[u_i] \quad E[\cancel{\beta_1}] = 0$$

$$= \beta_0 + \beta_1 \bar{x} - \hat{\beta}_1 \bar{x} = \beta_0 + \bar{x} (\beta_1 - \hat{\beta}_1) \quad \begin{aligned} &= \beta_0 + E[\beta_1] \bar{x} \\ &= \beta_0 + \beta_1 \bar{x} \end{aligned}$$

$$E[\hat{\beta}_0] = E[\beta_0 + \bar{x} (\beta_1 - \hat{\beta}_1)] = E[\beta_0] + \bar{x} \underbrace{E[\beta_1 - \hat{\beta}_1]}_0 = \beta_0$$

EX2

$$y = X\beta + u$$

$n \times 1 \quad n \times 1 \quad n \times 1 \quad n \times 1$

⑤ Homoskedasticity: $\text{Var}(u|x) = \sigma^2 I_n \quad \sigma^2 > 0$

$$\text{OLS } \hat{\beta} = (X'X)^{-1} X'y \quad ①$$

$$= (X'X)^{-1} X'(X\beta + u) = \cancel{(X'X)^{-1} X'X} \beta + (X'X)^{-1} X'u$$

unbiasedness

$$E[\hat{\beta}] = E[\cancel{(X'X)^{-1} X'X} \beta + (X'X)^{-1} X'u] = E[\beta] + E[\cancel{(X'X)^{-1} X'} X'u]$$

$$= \beta + (X'X)^{-1} X'E[u]$$

$$\underbrace{E[\hat{\beta}]}_{= \beta} = \beta \quad \underbrace{E[u]}_0$$

variance of $\hat{\beta}$

$$\text{Var}(\hat{\beta}) = \text{Var}((X'X)^{-1} X'u) = (X'X)^{-1} X' \text{Var}(u) X (X'X)^{-1}$$

⑤ $\sigma^2 I_n$